Monotype_open_preservation and ind fixes

TabularTypeInterpreter/F⊗⊕ω/Semantics/Environment/Basic.lean
@@ -59,20 +59,20 @@ x ≠ x'
 ───────────────── termVarExt
 x : A ∈ Δ, x' : B
 
-judgement_syntax a " ∈ " "dom" "(" Δ ")" : Environment.InTypeVarInDom (id a)
+judgement_syntax a " ∈ " "dom" "(" Δ ")" : Environment.TypeVarInDom (id a)
 
-def Environment.InTypeVarInDom a (Δ : Environment) := a ∈ Δ.typeVarDom
+def Environment.TypeVarInDom a (Δ : Environment) := a ∈ Δ.typeVarDom
 
-judgement_syntax a " ∉ " "dom" "(" Δ ")" : Environment.NotInTypeVarInDom (id a)
+judgement_syntax a " ∉ " "dom" "(" Δ ")" : Environment.TypeVarNotInDom (id a)
 
-def Environment.NotInTypeVarInDom a Δ := ¬[[a ∈ dom(Δ)]]
+def Environment.TypeVarNotInDom a Δ := ¬[[a ∈ dom(Δ)]]
 
-judgement_syntax x " ∈ " "dom" "(" Δ ")" : Environment.InTermVarInDom (id x)
+judgement_syntax x " ∈ " "dom" "(" Δ ")" : Environment.TermVarInDom (id x)
 
-def Environment.InTermVarInDom x (Δ : Environment) := x ∈ Δ.termVarDom
+def Environment.TermVarInDom x (Δ : Environment) := x ∈ Δ.termVarDom
 
-judgement_syntax x " ∉ " "dom" "(" Δ ")" : Environment.NotInTermVarInDom (id x)
+judgement_syntax x " ∉ " "dom" "(" Δ ")" : Environment.TermVarNotInDom (id x)
 
-def Environment.NotInTermVarInDom x Δ := ¬[[x ∈ dom(Δ)]]
+def Environment.TermVarNotInDom x Δ := ¬[[x ∈ dom(Δ)]]
 
 end TabularTypeInterpreter.«F⊗⊕ω»
