TabularTypeInterpreter/F⊗⊕ω/Lemmas/Environment/Basic.lean
@@ -1,6 +1,8 @@
 import TabularTypeInterpreter.«F⊗⊕ω».Semantics.Environment
 
-namespace TabularTypeInterpreter.«F⊗⊕ω».Environment
+namespace TabularTypeInterpreter.«F⊗⊕ω»
+
+namespace Environment
 
 theorem append_empty (Δ : Environment) : Δ.append empty = Δ := rfl
 
@@ -9,4 +11,34 @@ theorem empty_append (Δ : Environment) : append empty Δ = Δ := by
   | empty => rfl
   | typeExt Δ' .. | termExt Δ' .. => rw [append, Δ'.empty_append]
 
-end TabularTypeInterpreter.«F⊗⊕ω».Environment
+theorem typeVarDom_append : (append Δ Δ').typeVarDom = Δ'.typeVarDom ++ Δ.typeVarDom := by
+  match Δ' with
+  | empty => rw [append, typeVarDom, List.nil_append]
+  | typeExt .. => rw [append, typeVarDom, typeVarDom_append, typeVarDom, List.cons_append]
+  | termExt .. => rw [append, typeVarDom, typeVarDom_append, typeVarDom]
+
+end Environment
+
+namespace TypeVarInEnvironment
+
+theorem eq_of (aKinΔ : [[a : K ∈ Δ]]) : ∃ Δ' Δ'', Δ = [[(Δ', a : K, Δ'')]] := by
+  match aKinΔ with
+  | .head => exact ⟨_, .empty, rfl⟩
+  | .typeVarExt aKinΔ' _ =>
+    rcases aKinΔ'.eq_of with ⟨_, _, rfl⟩
+    rw [← Environment.append]
+    exact ⟨_, _, rfl⟩
+  | .termVarExt aKinΔ' =>
+    rcases aKinΔ'.eq_of with ⟨_, _, rfl⟩
+    rw [← Environment.append]
+    exact ⟨_, _, rfl⟩
+
+theorem TypeVarInDom_of (aKinΔ : [[a : K ∈ Δ]]) : [[a ∈ dom(Δ)]] :=
+  match aKinΔ with
+  | .head => .head _
+  | .typeVarExt aKinΔ' anea' => .tail _ aKinΔ'.TypeVarInDom_of
+  | .termVarExt aKinΔ' => aKinΔ'.TypeVarInDom_of
+
+end TypeVarInEnvironment
+
+end TabularTypeInterpreter.«F⊗⊕ω»
