TabularTypeInterpreter/F⊗⊕ω/Lemmas/Environment/EnvironmentWellFormedness.lean
@@ -2,22 +2,15 @@ import TabularTypeInterpreter.«F⊗⊕ω».Lemmas.Type
 import TabularTypeInterpreter.«F⊗⊕ω».Semantics.Environment
 
 theorem TabularTypeInterpreter.«F⊗⊕ω».EnvironmentWellFormedness.to_Kinding_of_TermVarIn
-  (Δwf : [[⊢ Δ]]) (xAinΔ : [[x : A ∈ Δ]]) : [[Δ ⊢ A : *]] := by match Δwf with
+  (Δwf : [[⊢ Δ]]) (xAinΔ : [[x : A ∈ Δ]]) : [[Δ ⊢ A : *]] := match Δwf with
   | .empty => nomatch xAinΔ
   | .typeVarExt Δ'wf aninΔ' (Δ := Δ') =>
     let .typeVarExt xAinΔ' := xAinΔ
-    rw [← Δ'.empty_append]
-    exact Δ'wf.to_Kinding_of_TermVarIn xAinΔ' |>.weakening (Δ'' := .typeExt .empty ..) <| by
-      rw [Environment.empty_append]
-      exact Δ'wf.typeVarExt aninΔ'
+    Δ'wf.to_Kinding_of_TermVarIn xAinΔ' |>.weakening (Δ' := .typeExt .empty ..) (Δ'' := .empty) <|
+      Δ'wf.typeVarExt aninΔ'
   | .termVarExt Δ'wf x'ninΔ' A'ki (Δ := Δ') => match xAinΔ with
     | .head =>
-      rw [← Δ'.empty_append]
-      exact A'ki.weakening (Δ'' := .termExt .empty ..) <| by
-        rw [Environment.empty_append]
-        exact Δ'wf.termVarExt x'ninΔ' A'ki
+      A'ki.weakening (Δ' := .termExt .empty ..) (Δ'' := .empty) <| Δ'wf.termVarExt x'ninΔ' A'ki
     | .termVarExt xAinΔ' _ =>
-      rw [← Δ'.empty_append]
-      exact Δ'wf.to_Kinding_of_TermVarIn xAinΔ' |>.weakening (Δ'' := .termExt .empty ..) <| by
-        rw [Environment.empty_append]
-        exact Δ'wf.termVarExt x'ninΔ' A'ki
+      Δ'wf.to_Kinding_of_TermVarIn xAinΔ' |>.weakening (Δ' := .termExt .empty ..) (Δ'' := .empty) <|
+        Δ'wf.termVarExt x'ninΔ' A'ki
