TabularTypeInterpreter/F⊗⊕ω/Lemmas/Type.lean
@@ -294,6 +294,10 @@ theorem TypeVar_open_eq {A : «Type»} (Alc : A.TypeVarLocallyClosed n) : A.Type
   | .prod .. => let .prod A'lc := Alc; rw [TypeVar_open, A'lc.TypeVar_open_eq]
   | .sum .. => let .sum A'lc := Alc; rw [TypeVar_open, A'lc.TypeVar_open_eq]
 
+theorem Type_open_id : TypeVarLocallyClosed A n → A.Type_open B n = A := by
+  induction A using rec_uniform generalizing n <;> aesop
+    (add simp [Type_open], safe cases TypeVarLocallyClosed, safe List.map_eq_id_of_eq_id_of_mem)
+
 theorem TypeVar_open_TypeVar_close_id
   : TypeVarLocallyClosed A n → (A.TypeVar_close a n).TypeVar_open a n = A := by
   induction A using rec_uniform generalizing n <;> aesop
@@ -371,11 +375,29 @@ theorem Type_open_dec (Alc : TypeVarLocallyClosed A (n + 1)) (Blc : B.TypeVarLoc
     let .sum A'lc := Alc
     exact sum <| A'lc.Type_open_dec Blc
 
+theorem Type_open_TypeVar_close_eq_TypeVar_subst
+  : TypeVarLocallyClosed A n → (A.TypeVar_close a n).Type_open B n = A.TypeVar_subst a B := by
+  induction A using rec_uniform generalizing n <;> aesop
+    (add simp [TypeVar_close, Type_open, TypeVar_subst], safe cases TypeVarLocallyClosed)
+
+private
+theorem Type_open_id' : TypeVarLocallyClosed A n → A = A.Type_open B n := (Type_open_id · |>.symm)
+
+theorem Type_open_TypeVar_subst_dist
+  : TypeVarLocallyClosed B' n → (Type_open A B n).TypeVar_subst a B' =
+    (A.TypeVar_subst a B').Type_open (B.TypeVar_subst a B') n := by
+  induction A using rec_uniform generalizing n <;> aesop
+    (add simp [Type_open, TypeVar_subst], 40% Type_open_id', 40% weaken)
+
 end TypeVarLocallyClosed
 
 theorem TypeVar_close_eq_of_not_mem_freeTypeVars
   : a ∉ freeTypeVars A → A.TypeVar_close a n = A := by
   induction A using rec_uniform generalizing n <;> aesop (add simp [freeTypeVars, TypeVar_close])
+
+theorem TypeVar_subst_id_of_not_mem_freeTypeVars
+  : a ∉ freeTypeVars A → A.TypeVar_subst a B = A := by
+  induction A using rec_uniform <;> aesop (add simp [freeTypeVars, TypeVar_subst])
 
 theorem TypeVar_close_TypeVar_open_eq_of_not_mem_freeTypeVars
   : a ∉ freeTypeVars A → (A.TypeVar_open a n).TypeVar_close a n = A := by
@@ -398,6 +420,16 @@ theorem TypeVar_open_inj_of_not_mem_freeTypeVars (aninA : a ∉ freeTypeVars A)
 theorem not_mem_freeTypeVars_TypeVar_close : a ∉ (TypeVar_close A a n).freeTypeVars := by
   induction A using rec_uniform generalizing n <;> aesop
     (add simp [TypeVar_close, freeTypeVars], safe cases TypeVar)
+
+theorem not_mem_freeTypeVars_TypeVar_open_intro
+  : a ∉ freeTypeVars A → a ≠ a' → a ∉ (A.TypeVar_open a' n).freeTypeVars := by
+  induction A using rec_uniform generalizing n <;> aesop
+    (add simp [TypeVar_open, freeTypeVars], safe cases TypeVar)
+
+theorem not_mem_freeTypeVars_TypeVar_open_drop
+  : a ∉ (TypeVar_open A a' n).freeTypeVars → a ∉ A.freeTypeVars := by
+  induction A using rec_uniform generalizing n <;> aesop
+    (add simp [TypeVar_open, freeTypeVars], safe cases TypeVar)
 
 end «Type»
 
@@ -431,16 +463,54 @@ theorem TypeVarLocallyClosed_of : [[Δ ⊢ A : K]] → A.TypeVarLocallyClosed 0 
   | .sum A', .sum A'opki => .sum A'opki.TypeVarLocallyClosed_of
 termination_by sizeOf A
 decreasing_by
-  all_goals (simp; try simp_arith)
+  all_goals simp_arith
   rw [List.map_singleton_flatten]
   apply Nat.le_of_lt
   exact List.sizeOf_lt_of_mem A'''in
+
+theorem not_mem_freeTypeVars_of (Aki : [[Δ ⊢ A : K]]) (aninΔ : [[a ∉ dom(Δ)]])
+  : a ∉ A.freeTypeVars := by match Aki with
+  | .var a'inΔ =>
+    rw [Type.freeTypeVars]
+    apply List.not_mem_singleton.mpr
+    intro aeqa'
+    cases aeqa'
+    nomatch aninΔ a'inΔ.TypeVarInDom_of
+  | .lam I A'opki | .scheme I A'opki =>
+    let ⟨a', a'nin⟩ := a :: I |>.exists_fresh
+    let ⟨a'nea, a'ninI⟩ := List.not_mem_cons.mp a'nin
+    rw [Type.freeTypeVars]
+    exact Type.not_mem_freeTypeVars_TypeVar_open_drop <|
+      A'opki a' a'ninI |>.not_mem_freeTypeVars_of (List.not_mem_cons.mpr ⟨a'nea.symm, aninΔ⟩)
+  | .app A'ki Bki | .arr A'ki Bki | .listApp A'ki Bki =>
+
+    rw [Type.freeTypeVars]
+    exact List.not_mem_append'.mpr ⟨
+      A'ki.not_mem_freeTypeVars_of aninΔ,
+      Bki.not_mem_freeTypeVars_of aninΔ
+    ⟩
+  | .list Aski =>
+    rw [Type.freeTypeVars, List.mapMem_eq_map, List.map_singleton_flatten, List.map_map]
+    apply List.not_mem_flatten.mpr
+    intro as mem
+    let ⟨i, mem', eq⟩ := Std.Range.mem_of_mem_map mem
+    cases eq
+    exact Aski i mem' |>.not_mem_freeTypeVars_of aninΔ
+  | .prod A'ki | .sum A'ki =>
+    rw [Type.freeTypeVars]
+    exact A'ki.not_mem_freeTypeVars_of aninΔ
+termination_by sizeOf A
+decreasing_by
+  all_goals simp_arith
+  rw [List.map_singleton_flatten]
+  apply Nat.le_of_lt
+  exact List.sizeOf_lt_of_mem <| Std.Range.mem_map_of_mem mem'
 
 theorem Type_open_preservation {A : «Type»}
   (Aki : Kinding [[(Δ, a : K, Δ')]] (A.TypeVar_open a n) K') (aninfvA : a ∉ A.freeTypeVars)
   (Bki : [[Δ ⊢ B : K]]) : Kinding [[(Δ, (Δ' [B / a]))]] (A.Type_open B n) K' := sorry
 
-theorem weakening : [[Δ ⊢ A : K]] → [[⊢ Δ', Δ, Δ'']] → [[Δ', Δ, Δ'' ⊢ A : K]] := sorry
+theorem weakening : [[Δ, Δ'' ⊢ A : K]] → [[⊢ Δ, Δ', Δ'']] → [[Δ, Δ', Δ'' ⊢ A : K]] := sorry
 
 theorem unit : [[Δ ⊢ ⊗ { } : *]] := by
   have := list (Δ := Δ) (A := fun _ => .list []) (K := .star) (n := 0) (fun _ => nomatch ·)
@@ -457,17 +527,13 @@ theorem prj_evidence (Δwf : [[⊢ Δ]]) (A₀ki : [[Δ ⊢ A₀ : L K]]) (A₁k
   · apply prod
     apply listApp
     · exact var .head
-    · rw [A₁ki.TypeVarLocallyClosed_of.TypeVar_open_eq, ← Δ.empty_append]
-      apply A₁ki.weakening (Δ' := .empty) (Δ'' := .typeExt .empty a _)
-      rw [Environment.empty_append]
-      exact Δwf.typeVarExt anin
+    · rw [A₁ki.TypeVarLocallyClosed_of.TypeVar_open_eq]
+      exact A₁ki.weakening (Δ' := .typeExt .empty a _) (Δ'' := .empty) <| Δwf.typeVarExt anin
   · apply prod
     apply listApp
     · exact var .head
-    · rw [A₀ki.TypeVarLocallyClosed_of.TypeVar_open_eq, ← Δ.empty_append]
-      apply A₀ki.weakening (Δ' := .empty) (Δ'' := .typeExt .empty a _)
-      rw [Environment.empty_append]
-      exact Δwf.typeVarExt anin
+    · rw [A₀ki.TypeVarLocallyClosed_of.TypeVar_open_eq]
+      exact A₀ki.weakening (Δwf.typeVarExt anin) (Δ' := .typeExt .empty a _) (Δ'' := .empty)
 
 theorem inj_evidence (Δwf : [[⊢ Δ]]) (A₀ki : [[Δ ⊢ A₀ : L K]]) (A₁ki : [[Δ ⊢ A₁ : L K]])
   : [[Δ ⊢ ∀ a : K ↦ *. (⊕ (a$0 ⟦A₀⟧)) → ⊕ (a$0 ⟦A₁⟧) : *]] := by
@@ -478,17 +544,13 @@ theorem inj_evidence (Δwf : [[⊢ Δ]]) (A₀ki : [[Δ ⊢ A₀ : L K]]) (A₁k
   · apply sum
     apply listApp
     · exact var .head
-    · rw [A₀ki.TypeVarLocallyClosed_of.TypeVar_open_eq, ← Δ.empty_append]
-      apply A₀ki.weakening (Δ' := .empty) (Δ'' := .typeExt .empty a _)
-      rw [Environment.empty_append]
-      exact Δwf.typeVarExt anin
+    · rw [A₀ki.TypeVarLocallyClosed_of.TypeVar_open_eq]
+      exact A₀ki.weakening (Δ' := .typeExt .empty a _) (Δ'' := .empty) <| Δwf.typeVarExt anin
   · apply sum
     apply listApp
     · exact var .head
-    · rw [A₁ki.TypeVarLocallyClosed_of.TypeVar_open_eq, ← Δ.empty_append]
-      apply A₁ki.weakening (Δ' := .empty) (Δ'' := .typeExt .empty a _)
-      rw [Environment.empty_append]
-      exact Δwf.typeVarExt anin
+    · rw [A₁ki.TypeVarLocallyClosed_of.TypeVar_open_eq]
+      exact A₁ki.weakening (Δ' := .typeExt .empty a _) (Δ'' := .empty) <| Δwf.typeVarExt anin
 
 theorem concat_evidence (Δwf : [[⊢ Δ]]) (A₀ki : [[Δ ⊢ A₀ : L K]]) (A₁ki : [[Δ ⊢ A₁ : L K]])
   (A₂ki : [[Δ ⊢ A₂ : L K]])
@@ -500,25 +562,19 @@ theorem concat_evidence (Δwf : [[⊢ Δ]]) (A₀ki : [[Δ ⊢ A₀ : L K]]) (A�
   · apply prod
     apply listApp
     · exact var .head
-    · rw [A₀ki.TypeVarLocallyClosed_of.TypeVar_open_eq, ← Δ.empty_append]
-      apply A₀ki.weakening (Δ' := .empty) (Δ'' := .typeExt .empty a _)
-      rw [Environment.empty_append]
-      exact Δwf.typeVarExt anin
+    · rw [A₀ki.TypeVarLocallyClosed_of.TypeVar_open_eq]
+      exact A₀ki.weakening (Δ' := .typeExt .empty a _) (Δ'' := .empty) <| Δwf.typeVarExt anin
   · apply arr
     · apply prod
       apply listApp
       · exact var .head
-      · rw [A₁ki.TypeVarLocallyClosed_of.TypeVar_open_eq, ← Δ.empty_append]
-        apply A₁ki.weakening (Δ' := .empty) (Δ'' := .typeExt .empty a _)
-        rw [Environment.empty_append]
-        exact Δwf.typeVarExt anin
+      · rw [A₁ki.TypeVarLocallyClosed_of.TypeVar_open_eq]
+        exact A₁ki.weakening (Δ' := .typeExt .empty a _) (Δ'' := .empty) <| Δwf.typeVarExt anin
     · apply prod
       apply listApp
       · exact var .head
-      · rw [A₂ki.TypeVarLocallyClosed_of.TypeVar_open_eq, ← Δ.empty_append]
-        apply A₂ki.weakening (Δ' := .empty) (Δ'' := .typeExt .empty a _)
-        rw [Environment.empty_append]
-        exact Δwf.typeVarExt anin
+      · rw [A₂ki.TypeVarLocallyClosed_of.TypeVar_open_eq]
+        exact A₂ki.weakening (Δ' := .typeExt .empty a _) (Δ'' := .empty) <| Δwf.typeVarExt anin
 
 theorem elim_evidence (Δwf : [[⊢ Δ]]) (A₀ki : [[Δ ⊢ A₀ : L K]]) (A₁ki : [[Δ ⊢ A₁ : L K]])
   (A₂ki : [[Δ ⊢ A₂ : L K]])
@@ -536,10 +592,9 @@ theorem elim_evidence (Δwf : [[⊢ Δ]]) (A₀ki : [[Δ ⊢ A₀ : L K]]) (A₁
       apply listApp
       · exact var <| .typeVarExt .head aₜnea.symm
       · let A₀lc := A₀ki.TypeVarLocallyClosed_of
-        rw [A₀lc.weaken (n := 1) |>.TypeVar_open_eq, A₀lc.TypeVar_open_eq, ← Δ.empty_append]
-        apply A₀ki.weakening (Δ' := .empty) (Δ'' := .typeExt (.typeExt .empty a _) aₜ _)
-        rw [Environment.empty_append]
-        exact Δwf.typeVarExt anin |>.typeVarExt aₜnin
+        rw [A₀lc.weaken (n := 1) |>.TypeVar_open_eq, A₀lc.TypeVar_open_eq]
+        exact A₀ki.weakening (Δ' := .typeExt (.typeExt .empty a _) aₜ _) (Δ'' := .empty) <|
+          Δwf.typeVarExt anin |>.typeVarExt aₜnin
     · exact var .head
   · apply arr
     · apply arr
@@ -547,26 +602,134 @@ theorem elim_evidence (Δwf : [[⊢ Δ]]) (A₀ki : [[Δ ⊢ A₀ : L K]]) (A₁
         apply listApp
         · exact var <| .typeVarExt .head aₜnea.symm
         · let A₁lc := A₁ki.TypeVarLocallyClosed_of
-          rw [A₁lc.weaken (n := 1) |>.TypeVar_open_eq, A₁lc.TypeVar_open_eq, ← Δ.empty_append]
-          apply A₁ki.weakening (Δ' := .empty) (Δ'' := .typeExt (.typeExt .empty a _) aₜ _)
-          rw [Environment.empty_append]
-          exact Δwf.typeVarExt anin |>.typeVarExt aₜnin
+          rw [A₁lc.weaken (n := 1) |>.TypeVar_open_eq, A₁lc.TypeVar_open_eq]
+          exact A₁ki.weakening (Δ' := .typeExt (.typeExt .empty a _) aₜ _) (Δ'' := .empty) <|
+            Δwf.typeVarExt anin |>.typeVarExt aₜnin
       · exact var .head
     · apply arr
       · apply sum
         apply listApp
         · exact var <| .typeVarExt .head aₜnea.symm
         · let A₂lc := A₂ki.TypeVarLocallyClosed_of
-          rw [A₂lc.weaken (n := 1) |>.TypeVar_open_eq, A₂lc.TypeVar_open_eq, ← Δ.empty_append]
-          apply A₂ki.weakening (Δ' := .empty) (Δ'' := .typeExt (.typeExt .empty a _) aₜ _)
-          rw [Environment.empty_append]
-          exact Δwf.typeVarExt anin |>.typeVarExt aₜnin
+          rw [A₂lc.weaken (n := 1) |>.TypeVar_open_eq, A₂lc.TypeVar_open_eq]
+          exact A₂ki.weakening (Δ' := .typeExt (.typeExt .empty a _) aₜ _) (Δ'' := .empty) <|
+            Δwf.typeVarExt anin |>.typeVarExt aₜnin
       · exact var .head
 
+local instance : Inhabited «Type» where
+  default := .list []
+in
 theorem ind_evidence (Δwf : [[⊢ Δ]])
-  (Bᵣki : [[Δ, aₗ : *, aₜ : K, aₚ : L K, aᵢ : L K, aₙ : L K ⊢ Bᵣ^aₙ^aᵢ^aₚ^aₜ^aₗ : *]])
-  (Bₗki : [[Δ, aᵢ : L K, aₙ : L K ⊢ Bₗ^aₙ^aᵢ : *]])
-  : [[Δ ⊢ ∀ aₘ : (L K) ↦ *. (∀ aₗ : *. ∀ aₜ : K. ∀ aₚ : L K. ∀ aᵢ : L K. ∀ aₙ : L K. Bᵣ → Bₗ → aₗ$4 → aₘ$5 aₚ$2 → aₘ$5 aₙ$0) → aₘ$5 { } → aₘ$5 A : *]] := sorry
+  (Aki : [[Δ ⊢ A : L K]])
+  (Bᵣki : ∀ aₗ ∉ I₀, ∀ aₜ ∉ aₗ :: I₀, ∀ aₚ ∉ aₜ :: aₗ :: I₀, ∀ aᵢ ∉ aₚ :: aₜ :: aₗ :: I₀, ∀ aₙ ∉ aᵢ :: aₚ :: aₜ :: aₗ :: I₀,
+    [[Δ, aₗ : *, aₜ : K, aₚ : L K, aᵢ : L K, aₙ : L K ⊢ Bᵣ^aₗ#4^aₜ#3^aₚ#2^aᵢ#1^aₙ : *]])
+  (Bₗki : ∀ aᵢ ∉ I₁, ∀ aₙ ∉ aᵢ :: I₁, [[Δ, aᵢ : L K, aₙ : L K ⊢ Bₗ^aᵢ#1^aₙ : *]])
+  : [[Δ ⊢ ∀ aₘ : (L K) ↦ *. (∀ aₗ : *. ∀ aₜ : K. ∀ aₚ : L K. ∀ aᵢ : L K. ∀ aₙ : L K. Bᵣ → Bₗ → aₗ$4 → (aₘ$5 aₚ$2) → aₘ$5 aₙ$0) → (aₘ$0 { }) → aₘ$0 A : *]] := by
+  apply scheme Δ.typeVarDom
+  intro aₘ aₘnin
+  let Δaₘwf := Δwf.typeVarExt aₘnin (K := K.list.arr .star)
+  simp [Type.TypeVar_open]
+  let ⟨aₗ, aₗnin⟩ := I₀.exists_fresh
+  let ⟨aₜ, aₜnin⟩ := aₗ :: I₀ |>.exists_fresh
+  let ⟨aₚ, aₚnin⟩ := aₜ :: aₗ :: I₀ |>.exists_fresh
+  let ⟨aᵢ, aᵢnin⟩ := aₚ :: aₜ :: aₗ :: I₀ |>.exists_fresh
+  let ⟨aₙ, aₙnin⟩ := aᵢ :: aₚ :: aₜ :: aₗ :: I₀ |>.exists_fresh
+  let Bᵣlc := Bᵣki _ aₗnin _ aₜnin _ aₚnin _ aᵢnin _ aₙnin
+    |>.TypeVarLocallyClosed_of.weaken (n := 5)
+    |>.TypeVar_open_drop (Nat.lt.step <| Nat.lt.step <| Nat.lt.step <| Nat.lt.step <| .base _)
+    |>.TypeVar_open_drop (Nat.lt.step <| Nat.lt.step <| Nat.lt.step <| .base _)
+    |>.TypeVar_open_drop (Nat.lt.step <| Nat.lt.step <| .base _)
+    |>.TypeVar_open_drop (Nat.lt.step <| .base _)
+    |>.TypeVar_open_drop (Nat.lt.base _)
+  let ⟨aᵢ, aᵢnin⟩ := I₁ |>.exists_fresh
+  let ⟨aₙ, aₙnin⟩ := aᵢ :: I₁ |>.exists_fresh
+  let Bₗlc := Bₗki _ aᵢnin _ aₙnin |>.TypeVarLocallyClosed_of.weaken (n := 2)
+    |>.TypeVar_open_drop (Nat.lt.step <| .base _) |>.TypeVar_open_drop (Nat.lt.base _)
+  rw [Aki.TypeVarLocallyClosed_of.TypeVar_open_eq, Bᵣlc.TypeVar_open_eq,
+      Bₗlc.weaken (n := 3).TypeVar_open_eq]
+  apply arr
+  · apply scheme <| I₀ ++ aₘ :: Δ.typeVarDom
+    intro aₗ aₗnin
+    let ⟨aₗninI₀, aₗninΔ⟩ := List.not_mem_append'.mp aₗnin
+    let Δaₘaₗwf := Δaₘwf.typeVarExt aₗninΔ (K := .star)
+    let aₘneaₗ := List.ne_of_not_mem_cons aₗninΔ
+    symm at aₘneaₗ
+    simp [Type.TypeVar_open]
+    rw [Bₗlc.weaken (n := 2).TypeVar_open_eq]
+    apply scheme <| aₗ :: I₀ ++ aₗ :: aₘ :: Δ.typeVarDom
+    intro aₜ aₜnin
+    let ⟨aₜninI₀, aₜninΔ⟩ := List.not_mem_append'.mp aₜnin
+    let Δaₘaₗaₜwf := Δaₘaₗwf.typeVarExt aₜninΔ (K := K)
+    let aₗneaₜ := List.ne_of_not_mem_cons aₜninI₀
+    let aₘneaₜ := List.ne_of_not_mem_cons <| List.not_mem_of_not_mem_cons <| aₜninΔ
+    symm at aₗneaₜ aₘneaₜ
+    simp [Type.TypeVar_open]
+    rw [Bₗlc.weaken (n := 1).TypeVar_open_eq]
+    apply scheme <| aₜ :: aₗ :: I₀ ++ aₜ :: aₗ :: aₘ :: Δ.typeVarDom
+    intro aₚ aₚnin
+    let ⟨aₚninI₀, aₚninΔ⟩ := List.not_mem_append'.mp aₚnin
+    let Δaₘaₗaₜaₚwf := Δaₘaₗaₜwf.typeVarExt aₚninΔ (K := K.list)
+    let aₗneaₚ := List.ne_of_not_mem_cons <| List.not_mem_of_not_mem_cons <| aₚninI₀
+    let aₘneaₚ := List.ne_of_not_mem_cons <| List.not_mem_of_not_mem_cons <|
+      List.not_mem_of_not_mem_cons <| aₚninΔ
+    symm at aₗneaₚ aₘneaₚ
+    simp [Type.TypeVar_open]
+    rw [Bₗlc.TypeVar_open_eq]
+    apply scheme <| aₚ :: aₜ :: aₗ :: I₀ ++ I₁ ++ aₚ :: aₜ :: aₗ :: aₘ :: Δ.typeVarDom
+    intro aᵢ aᵢnin
+    let ⟨aᵢninI₀I₁, aᵢninΔ⟩ := List.not_mem_append'.mp aᵢnin
+    let ⟨aᵢninI₀, aᵢninI₁⟩ := List.not_mem_append'.mp aᵢninI₀I₁
+    let aₚneaᵢ := List.ne_of_not_mem_cons aᵢninI₀
+    let Δaₘaₗaₜaₚaᵢwf := Δaₘaₗaₜaₚwf.typeVarExt aᵢninΔ (K := K.list)
+    let aₗneaᵢ := List.ne_of_not_mem_cons <| List.not_mem_of_not_mem_cons <|
+      List.not_mem_of_not_mem_cons <| aᵢninI₀
+    let aₘneaᵢ := List.ne_of_not_mem_cons <| List.not_mem_of_not_mem_cons <|
+      List.not_mem_of_not_mem_cons <| List.not_mem_of_not_mem_cons <| aᵢninΔ
+    symm at aₚneaᵢ aₗneaᵢ aₘneaᵢ
+    simp [Type.TypeVar_open]
+    apply scheme <|
+      aᵢ :: aₚ :: aₜ :: aₗ :: I₀ ++ aᵢ :: I₁ ++ aᵢ :: aₚ :: aₜ :: aₗ :: aₘ :: Δ.typeVarDom
+    intro aₙ aₙnin
+    let ⟨aₙninI₀I₁, aₙninΔ⟩ := List.not_mem_append'.mp aₙnin
+    let ⟨aₙninI₀, aₙninI₁⟩ := List.not_mem_append'.mp aₙninI₀I₁
+    let Δaₘaₗaₜaₚaᵢaₙwf := Δaₘaₗaₜaₚaᵢwf.typeVarExt aₙninΔ (K := K.list)
+    let aₚneaₙ := List.ne_of_not_mem_cons <| List.not_mem_of_not_mem_cons aₙninI₀
+    let aₗneaₙ := List.ne_of_not_mem_cons <| List.not_mem_of_not_mem_cons <|
+      List.not_mem_of_not_mem_cons <| List.not_mem_of_not_mem_cons <| aₙninI₀
+    let aₘneaₙ := List.ne_of_not_mem_cons <| List.not_mem_of_not_mem_cons <|
+      List.not_mem_of_not_mem_cons <| List.not_mem_of_not_mem_cons <|
+      List.not_mem_of_not_mem_cons <| aₙninΔ
+    symm at aₚneaₙ aₗneaₙ aₘneaₙ
+    simp [Type.TypeVar_open]
+    apply arr <| Bᵣki _ aₗninI₀ _ aₜninI₀ _ aₚninI₀ _ aᵢninI₀ _ aₙninI₀ |>.weakening Δaₘaₗaₜaₚaᵢaₙwf
+      (Δ := Δ)
+      (Δ' := .typeExt .empty ..)
+      (Δ'' := .typeExt (.typeExt (.typeExt (.typeExt (.typeExt .empty ..) ..) ..) ..) ..)
+    apply arr <| Bₗki _ aᵢninI₁ _ aₙninI₁ |>.weakening Δaₘaₗaₜaₚaᵢaₙwf
+      (Δ := Δ)
+      (Δ' := .typeExt (.typeExt (.typeExt (.typeExt .empty ..) ..) ..) ..)
+      (Δ'' := .typeExt (.typeExt .empty ..) ..)
+    · apply arr
+      · exact var <|
+          .typeVarExt (.typeVarExt (.typeVarExt (.typeVarExt .head aₗneaₜ) aₗneaₚ) aₗneaᵢ) aₗneaₙ
+      · apply arr
+        · apply app
+          · exact var <| .typeVarExt (.typeVarExt (.typeVarExt
+               (.typeVarExt (.typeVarExt .head aₘneaₗ) aₘneaₜ) aₘneaₚ) aₘneaᵢ) aₘneaₙ
+          · exact var <| .typeVarExt (.typeVarExt .head aₚneaᵢ) aₚneaₙ
+        · apply app
+          · exact var <| .typeVarExt (.typeVarExt (.typeVarExt
+               (.typeVarExt (.typeVarExt .head aₘneaₗ) aₘneaₜ) aₘneaₚ) aₘneaᵢ) aₘneaₙ
+          · exact var .head
+  · apply arr
+    · apply app
+      · exact var .head
+      · rw [← Std.Range.map_get!_eq (as := []), Std.Range.map, ← List.map_singleton_flatten,
+            ← Std.Range.map]
+        exact list fun _ => (nomatch ·)
+    · apply app
+      · exact var .head
+      · exact Aki.weakening (Δ' := .typeExt .empty ..) (Δ'' := .empty) Δaₘwf
 
 end Kinding
 
